move

Foundation/IntProp/Hilbert/Basic.lean
@@ -1,44 +1,34 @@
 import Foundation.Logic.HilbertStyle.Supplemental
-import Foundation.IntProp.Formula
+import Foundation.IntProp.Substitution
 
 namespace LO.IntProp
 
 variable {α : Type u}
 
 structure Hilbert (α) where
-  axioms : Theory α
+  axioms : Set (Formula α)
 
 namespace Hilbert
 
+abbrev axiomInstances (H : Hilbert α) : Set (Formula α) := { φ⟦s⟧ | (φ ∈ H.axioms) (s : Substitution α) }
+
+class FiniteAxiomatizable (H : Hilbert α) where
+  axioms_fin : Set.Finite H.axioms := by simp
+
 variable {H : Hilbert α}
 
-
-section
-
-class IncludeEFQ (H : Hilbert α) where
-  include_EFQ : 𝗘𝗙𝗤 ⊆ H.axioms := by simp
-
-class IncludeLEM (H : Hilbert α) where
-  include_LEM : 𝗟𝗘𝗠 ⊆ H.axioms := by simp
-
-class IncludeDNE (H : Hilbert α) where
-  include_DNE : 𝗗𝗡𝗘 ⊆ H.axioms := by simp
-
-end
-
-
 inductive Deduction (H : Hilbert α) : Formula α → Type _
-  | eaxm {φ}     : φ ∈ H.axioms → Deduction H φ
-  | mdp {φ ψ}    : Deduction H (φ ➝ ψ) → Deduction H φ → Deduction H ψ
-  | verum        : Deduction H $ ⊤
-  | imply₁ φ ψ   : Deduction H $ φ ➝ ψ ➝ φ
-  | imply₂ φ ψ χ : Deduction H $ (φ ➝ ψ ➝ χ) ➝ (φ ➝ ψ) ➝ φ ➝ χ
-  | and₁ φ ψ     : Deduction H $ φ ⋏ ψ ➝ φ
-  | and₂ φ ψ     : Deduction H $ φ ⋏ ψ ➝ ψ
-  | and₃ φ ψ     : Deduction H $ φ ➝ ψ ➝ φ ⋏ ψ
-  | or₁ φ ψ      : Deduction H $ φ ➝ φ ⋎ ψ
-  | or₂ φ ψ      : Deduction H $ ψ ➝ φ ⋎ ψ
-  | or₃ φ ψ χ    : Deduction H $ (φ ➝ χ) ➝ (ψ ➝ χ) ➝ (φ ⋎ ψ ➝ χ)
+  | eaxm {φ}      : φ ∈ H.axiomInstances → Deduction H φ
+  | mdp {φ ψ}     : Deduction H (φ ➝ ψ) → Deduction H φ → Deduction H ψ
+  | verum         : Deduction H $ ⊤
+  | implyS φ ψ    : Deduction H $ φ ➝ ψ ➝ φ
+  | implyK φ ψ χ  : Deduction H $ (φ ➝ ψ ➝ χ) ➝ (φ ➝ ψ) ➝ φ ➝ χ
+  | andElimL φ ψ  : Deduction H $ φ ⋏ ψ ➝ φ
+  | andElimR φ ψ  : Deduction H $ φ ⋏ ψ ➝ ψ
+  | andIntro φ ψ  : Deduction H $ φ ➝ ψ ➝ φ ⋏ ψ
+  | orIntroL φ ψ  : Deduction H $ φ ➝ φ ⋎ ψ
+  | orIntroR φ ψ  : Deduction H $ ψ ➝ φ ⋎ ψ
+  | orElim φ ψ χ  : Deduction H $ (φ ➝ χ) ➝ (ψ ➝ χ) ➝ (φ ⋎ ψ ➝ χ)
 
 instance : System (Formula α) (Hilbert α) := ⟨Deduction⟩
 
@@ -49,157 +39,93 @@ section
 
 instance : System.ModusPonens H := ⟨mdp⟩
 
-instance : System.HasAxiomImply₁ H := ⟨imply₁⟩
+instance : System.HasAxiomImply₁ H := ⟨implyS⟩
 
-instance : System.HasAxiomImply₂ H := ⟨imply₂⟩
+instance : System.HasAxiomImply₂ H := ⟨implyK⟩
 
-instance : System.HasAxiomAndInst H := ⟨and₃⟩
+instance : System.HasAxiomAndInst H := ⟨andIntro⟩
 
 instance : System.Minimal H where
   mdp := mdp
   verum := verum
-  and₁ := and₁
-  and₂ := and₂
-  and₃ := and₃
-  or₁ := or₁
-  or₂ := or₂
-  or₃ := or₃
+  and₁ := andElimL
+  and₂ := andElimR
+  and₃ := andIntro
+  or₁ := orIntroL
+  or₂ := orIntroR
+  or₃ := orElim
 
-instance [H.IncludeEFQ] : System.HasAxiomEFQ H where
-  efq _ := eaxm $ Set.mem_of_subset_of_mem IncludeEFQ.include_EFQ (by simp);
+namespace Deduction
 
-instance [H.IncludeLEM] : System.HasAxiomLEM H where
-  lem _ := eaxm $ Set.mem_of_subset_of_mem IncludeLEM.include_LEM (by simp);
+lemma eaxm! {φ} (h : φ ∈ H.axiomInstances) : H ⊢! φ := ⟨eaxm h⟩
 
-instance [H.IncludeDNE] : System.HasAxiomDNE H where
-  dne _ := eaxm $ Set.mem_of_subset_of_mem IncludeDNE.include_DNE (by simp);
+open System
 
-instance [H.IncludeEFQ] : System.Intuitionistic H where
+noncomputable def rec!
+  {motive      : (φ : Formula α) → H ⊢! φ → Sort*}
+  (maxm       : ∀ {φ}, (h : φ ∈ H.axiomInstances) → motive φ (eaxm! h))
+  (mdp        : ∀ {φ ψ}, {hpq : H ⊢! φ ➝ ψ} → {hp : H ⊢! φ} → motive (φ ➝ ψ) hpq → motive φ hp → motive ψ (mdp! hpq hp))
+  (verum      : motive ⊤ verum!)
+  (implyS     : ∀ {φ ψ},   motive (Axioms.Imply₁ φ ψ) $ ⟨implyS φ ψ⟩)
+  (implyK     : ∀ {φ ψ χ}, motive (Axioms.Imply₂ φ ψ χ) $ ⟨implyK φ ψ χ⟩)
+  (andElimL   : ∀ {φ ψ},   motive (φ ⋏ ψ ➝ φ) $ ⟨andElimL φ ψ⟩)
+  (andElimR   : ∀ {φ ψ},   motive (φ ⋏ ψ ➝ ψ) $ ⟨andElimR φ ψ⟩)
+  (andIntro   : ∀ {φ ψ},   motive (φ ➝ ψ ➝ φ ⋏ ψ) $ ⟨andIntro φ ψ⟩)
+  (orIntroL   : ∀ {φ ψ},   motive (φ ➝ φ ⋎ ψ) $ ⟨orIntroL φ ψ⟩)
+  (orIntroR   : ∀ {φ ψ},   motive (ψ ➝ φ ⋎ ψ) $ ⟨orIntroR φ ψ⟩)
+  (orElim     : ∀ {φ ψ χ}, motive ((φ ➝ χ) ➝ (ψ ➝ χ) ➝ φ ⋎ ψ ➝ χ) $ ⟨orElim φ ψ χ⟩)
+  : ∀ {φ}, (d : H ⊢! φ) → motive φ d := by
+  intro φ d;
+  induction d.some with
+  | eaxm h => exact maxm h
+  | mdp hpq hp ihpq ihp => exact mdp (ihpq ⟨hpq⟩) (ihp ⟨hp⟩)
+  | _ => aesop
 
-instance [H.IncludeDNE] : System.Classical H where
+def subst! {φ} (s) (h : H ⊢! φ) : H ⊢! φ⟦s⟧ := by
+  induction h using Deduction.rec! with
+  | mdp ihφψ ihφ => exact ihφψ ⨀ ihφ;
+  | maxm h =>
+    obtain ⟨ψ, h, ⟨s', rfl⟩⟩ := h;
+    apply eaxm!;
+    use ψ;
+    constructor;
+    . assumption;
+    . use s' ∘ s;
+      exact subst_comp;
+  | _ => simp;
+
+end Deduction
 
 end
 
 
-abbrev theorems (H : Hilbert α) : Set (Formula α) := System.theory H
-
-
-section systems
-
-variable (α)
-
-protected abbrev Minimal : Hilbert α := ⟨∅⟩
-
-protected abbrev Int : Hilbert α := ⟨𝗘𝗙𝗤⟩
-instance : IncludeEFQ (Hilbert.Int α) where
-instance : System.Intuitionistic (Hilbert.Int α) where
-
-protected abbrev Cl : Hilbert α := ⟨𝗘𝗙𝗤 ∪ 𝗟𝗘𝗠⟩
-instance : IncludeLEM (α := α) (Hilbert.Cl α) where
-instance : IncludeEFQ (α := α) (Hilbert.Cl α) where
-
-/--
-  `KC` from Chagrov & Zakharyaschev (1997)
--/
-protected abbrev KC : Hilbert α := ⟨𝗘𝗙𝗤 ∪ 𝗪𝗟𝗘𝗠⟩
-instance : IncludeEFQ (α := α) (Hilbert.KC α) where
-instance : System.HasAxiomWeakLEM (Hilbert.KC α) where
-  wlem φ := by apply eaxm; aesop;
-
-/--
-  `LC` from Chagrov & Zakharyaschev (1997)
--/
-protected abbrev LC : Hilbert α := ⟨𝗘𝗙𝗤 ∪ 𝗗𝘂𝗺⟩
-instance : IncludeEFQ (α := α) (Hilbert.LC α) where
-instance : System.HasAxiomDummett (Hilbert.LC α) where
-  dummett φ ψ := by apply eaxm; aesop;
-
-
--- MEMO: Minimal <ₛ WeakMinimal <ₛ WeakClassical <ₛ Classical
-
-/--
-  `WeakMinimal` from Ariola (2007)
--/
-protected abbrev WeakMinimal : Hilbert α := ⟨𝗟𝗘𝗠⟩
-
-
-/--
-  `WeakClassical` from Ariola (2007)
--/
-protected abbrev WeakClassical : Hilbert α := ⟨𝗣𝗲⟩
-
-end systems
-
-
-abbrev Consistent (H : Hilbert α) := System.Consistent H
-
-
-namespace Deduction
-
-open System
-
-lemma eaxm! {H : Hilbert α} {φ : Formula α} (h : φ ∈ H.axioms) : H ⊢! φ := ⟨eaxm h⟩
-
-noncomputable def rec! {α : Type u} {H : Hilbert α}
-  {motive : (a : Formula α) → H ⊢! a → Sort u_1}
-  (eaxm   : ∀ {φ}, (a : φ ∈ H.axioms) → motive φ ⟨eaxm a⟩)
-  (mdp    : ∀ {φ ψ}, {hpq : H ⊢! (φ ➝ ψ)} → {hp : H ⊢! φ} → motive (φ ➝ ψ) hpq → motive φ hp → motive ψ (hpq ⨀ hp))
-  (verum  : motive ⊤ verum!)
-  (imply₁ : ∀ {φ ψ},   motive (φ ➝ ψ ➝ φ) imply₁!)
-  (imply₂ : ∀ {φ ψ χ}, motive ((φ ➝ ψ ➝ χ) ➝ (φ ➝ ψ) ➝ φ ➝ χ) imply₂!)
-  (and₁   : ∀ {φ ψ},   motive (φ ⋏ ψ ➝ φ) and₁!)
-  (and₂   : ∀ {φ ψ},   motive (φ ⋏ ψ ➝ ψ) and₂!)
-  (and₃   : ∀ {φ ψ},   motive (φ ➝ ψ ➝ φ ⋏ ψ) and₃!)
-  (or₁    : ∀ {φ ψ},   motive (φ ➝ φ ⋎ ψ) or₁!)
-  (or₂    : ∀ {φ ψ},   motive (ψ ➝ φ ⋎ ψ) or₂!)
-  (or₃    : ∀ {φ ψ χ}, motive ((φ ➝ χ) ➝ (ψ ➝ χ) ➝ φ ⋎ ψ ➝ χ) or₃!) :
-  {a : Formula α} → (t : H ⊢! a) → motive a t := by
-  intro φ d;
-  induction d.some with
-  | eaxm h => exact eaxm h
-  | mdp hpq hp ihpq ihp => exact mdp (ihpq ⟨hpq⟩) (ihp ⟨hp⟩)
-  | _ => aesop
-
-end Deduction
-
-
-open System
 
 section
 
-lemma weaker_than_of_subset_axiomset' {H₁ H₂ : Hilbert α} (hMaxm : ∀ {φ : Formula α}, φ ∈ H₁.axioms → H₂ ⊢! φ)
+open System
+
+variable {H₁ H₂ : Hilbert α}
+
+lemma weakerThan_of_dominate_axiomInstances (hMaxm : ∀ {φ : Formula α}, φ ∈ H₁.axiomInstances → H₂ ⊢! φ)
   : H₁ ≤ₛ H₂ := by
   apply System.weakerThan_iff.mpr;
   intro φ h;
   induction h using Deduction.rec! with
-  | eaxm hp => apply hMaxm hp;
+  | maxm hp => apply hMaxm hp;
   | mdp ihpq ihp => exact ihpq ⨀ ihp;
   | _ => simp;
 
-lemma weaker_than_of_subset_axiomset {H₁ H₂ : Hilbert α} (hSubset : H₁.axioms ⊆ H₂.axioms := by aesop) : H₁ ≤ₛ H₂ := by
-  apply weaker_than_of_subset_axiomset';
-  intro φ hp;
-  apply eaxm! $ hSubset hp;
-
-lemma Int_weaker_than_Cl : (Hilbert.Int α) ≤ₛ (Hilbert.Cl α) := weaker_than_of_subset_axiomset
-
-lemma Int_weaker_than_KC : (Hilbert.Int α) ≤ₛ (Hilbert.KC α) := weaker_than_of_subset_axiomset
-
-lemma Int_weaker_than_LC : (Hilbert.Int α) ≤ₛ (Hilbert.LC α) := weaker_than_of_subset_axiomset
-
-lemma KC_weaker_than_Cl : (Hilbert.KC α) ≤ₛ (Hilbert.Cl α) := weaker_than_of_subset_axiomset' $ by
-  rintro φ (⟨_, rfl⟩ | ⟨_, rfl⟩) <;> simp;
-
-lemma LC_weaker_than_Cl [DecidableEq α] : (Hilbert.LC α) ≤ₛ (Hilbert.Cl α) := by
-  apply weaker_than_of_subset_axiomset';
-  rintro φ (⟨_, rfl⟩ | ⟨_, _, rfl⟩) <;> simp;
-
-lemma KC_weaker_than_LC [DecidableEq α] : (Hilbert.KC α) ≤ₛ (Hilbert.LC α) := by
-  apply weaker_than_of_subset_axiomset';
-  rintro φ (⟨_, rfl⟩ | ⟨_, rfl⟩) <;> simp;
+lemma weakerThan_of_subset_axioms (hSubset : H₁.axioms ⊆ H₂.axioms)
+  : H₁ ≤ₛ H₂ := by
+  apply weakerThan_of_dominate_axiomInstances;
+  rintro φ ⟨ψ, hs, ⟨s, rfl⟩⟩;
+  apply eaxm!;
+  use ψ;
+  constructor;
+  . exact hSubset hs;
+  . use s;
 
 end
-
 
 end Hilbert
 
