Foundation/IntProp/Kripke/Basic.lean
@@ -1,9 +1,6 @@
 import Foundation.Vorspiel.BinaryRelations
 import Foundation.IntProp.Hilbert.Basic
 
-set_option autoImplicit false
-universe u v
-
 namespace LO.IntProp
 
 open System
@@ -13,53 +10,38 @@ namespace Kripke
 
 structure Frame where
   World : Type
-  Rel : Rel World World
   [world_nonempty : Nonempty World]
-  [rel_po : IsPartialOrder _ Rel]
+  Rel : Rel World World
+  rel_refl : Reflexive Rel
+  rel_trans : Transitive Rel
 
 instance : CoeSort Frame (Type) := ⟨Frame.World⟩
 instance : CoeFun Frame (λ F => F.World → F.World → Prop) := ⟨Frame.Rel⟩
 instance {F : Frame} : Nonempty F.World := F.world_nonempty
-instance {F : Frame} : IsPartialOrder _ F.Rel := F.rel_po
+-- instance {F : Frame} : IsPartialOrder _ F.Rel := F.rel_po
 
 abbrev Frame.Rel' {F : Frame} (x y : F.World) := F.Rel x y
 infix:45 " ≺ " => Frame.Rel'
 
 namespace Frame
 
-variable {F : Frame}
+variable {F : Frame} {x y z : F.World}
 
-@[trans] lemma rel_trans {x y z : F.World} : x ≺ y → y ≺ z → x ≺ z := IsTrans.trans x y z
-lemma rel_trans' : Transitive F.Rel := by apply rel_trans;
+@[refl, simp] lemma rel_refl' : x ≺ x := F.rel_refl x
 
-@[refl, simp] lemma rel_refl {x : F.World} : x ≺ x := IsRefl.refl x
-lemma rel_refl' : Reflexive F.Rel := by apply rel_refl
-
-@[simp] lemma rel_antisymm {x y : F.World} : x ≺ y → y ≺ x → x = y := IsAntisymm.antisymm x y
-lemma rel_antisymm' : AntiSymmetric F.Rel := by apply rel_antisymm
+@[trans] lemma rel_trans' : x ≺ y → y ≺ z → x ≺ z := by apply F.rel_trans
 
 end Frame
+
 
 abbrev pointFrame : Frame where
   World := Unit
   Rel := fun _ _ => True
+  rel_refl := by simp [Reflexive]
+  rel_trans := by simp [Transitive]
 
 
 abbrev FrameClass := Set (Frame)
-
-section
-
-abbrev AllFrameClass : FrameClass := Set.univ
-
-abbrev SymmetricFrameClass : FrameClass := { F : Kripke.Frame | Symmetric F }
-
-abbrev ConfluentFrameClass : FrameClass := { F : Kripke.Frame | Confluent F }
-
-abbrev ConnectedFrameClass : FrameClass := { F : Kripke.Frame | Connected F }
-
-abbrev EuclideanFrameClass : FrameClass := { F : Kripke.Frame | Euclidean F }
-
-end
 
 
 structure Valuation (F : Frame) where
@@ -132,15 +114,51 @@ lemma formula_hereditary
   | hor => simp_all [Satisfies]; tauto;
   | _ => simp_all [Satisfies];
 
-
 lemma neg_equiv : w ⊧ ∼φ ↔ w ⊧ φ ➝ ⊥ := by simp_all [Satisfies];
 
+lemma iff_subst_self {F : Frame} {V : Valuation F} {x : F.World} (s) :
+  letI U : Kripke.Valuation F := ⟨
+    λ w a => Satisfies ⟨F, V⟩ w ((.atom a)⟦s⟧),
+    fun {_ _} Rwv {_} => formula_hereditary Rwv
+  ⟩;
+  Satisfies ⟨F, U⟩ x φ ↔ Satisfies ⟨F, V⟩ x (φ⟦s⟧) := by
+  induction φ using Formula.rec' generalizing x with
+  | hatom a => simp [Satisfies];
+  | hfalsum => simp [Satisfies];
+  | himp φ ψ ihφ ihψ =>
+    constructor;
+    . intro hφψ y Rxy hφs;
+      apply ihψ.mp;
+      apply hφψ Rxy;
+      apply ihφ.mpr hφs;
+    . intro hφψs y Rxy hφ;
+      apply ihψ.mpr;
+      apply hφψs Rxy;
+      apply ihφ.mp hφ;
+  | hand φ ψ ihφ ihψ =>
+    constructor;
+    . rintro ⟨hφ, hψ⟩;
+      constructor;
+      . apply ihφ.mp hφ;
+      . apply ihψ.mp hψ;
+    . rintro ⟨hφ, hψ⟩;
+      apply Satisfies.and_def.mpr;
+      constructor;
+      . apply ihφ.mpr hφ;
+      . apply ihψ.mpr hψ;
+  | hor φ ψ ihφ ihψ =>
+    constructor;
+    . rintro (hφ | hψ);
+      . left; apply ihφ.mp hφ;
+      . right; apply ihψ.mp hψ;
+    . rintro (hφ | hψ);
+      . left; apply ihφ.mpr hφ;
+      . right; apply ihψ.mpr hψ;
 
 end Satisfies
 
 
 open Satisfies
-
 
 def ValidOnModel (M : Kripke.Model) (φ : Formula ℕ) := ∀ w : M.World, w ⊧ φ
 
@@ -152,7 +170,23 @@ variable {M : Model} {φ ψ χ : Formula ℕ}
 
 @[simp] protected lemma iff_models : M ⊧ φ ↔ Formula.Kripke.ValidOnModel M φ := iff_of_eq rfl
 
-@[simp] protected lemma verum : M ⊧ ⊤ := by simp [ValidOnModel, Satisfies];
+
+protected lemma verum : M ⊧ ⊤ := by simp [ValidOnModel, Satisfies];
+
+instance : Semantics.Top (Model) := ⟨λ _ => ValidOnModel.verum⟩
+
+
+protected lemma bot : ¬M ⊧ ⊥ := by simp [ValidOnModel, Satisfies];
+
+instance : Semantics.Bot (Model) := ⟨λ _ => ValidOnModel.bot⟩
+
+
+lemma iff_not_exists_world {M : Kripke.Model} : (¬M ⊧ φ) ↔ (∃ x : M.World, ¬x ⊧ φ) := by
+  apply not_iff_not.mp;
+  push_neg;
+  tauto;
+
+alias ⟨exists_world_of_not, not_of_exists_world⟩ := iff_not_exists_world
 
 protected lemma andElim₁ : M ⊧ φ ⋏ ψ ➝ φ := by simp_all [ValidOnModel, Satisfies];
 
@@ -168,7 +202,6 @@ protected lemma orInst₁ : M ⊧ φ ➝ φ ⋎ ψ := by simp_all [ValidOnModel,
 protected lemma orInst₂ : M ⊧ ψ ➝ φ ⋎ ψ := by simp_all [ValidOnModel, Satisfies];
 
 protected lemma orElim : M ⊧ (φ ➝ χ) ➝ (ψ ➝ χ) ➝ (φ ⋎ ψ ➝ χ) := by
-  simp_all only [ValidOnModel.iff_models, ValidOnModel, Satisfies.iff_models, Satisfies.imp_def, Satisfies.or_def];
   intro w₁ w₂ _ hpr w₃ hw₂₃ hqr w₄ hw₃₄ hpq;
   cases hpq with
   | inl hp => exact hpr (M.rel_trans hw₂₃ hw₃₄) hp;
@@ -180,67 +213,64 @@ protected lemma imply₁ : M ⊧ φ ➝ ψ ➝ φ := by
 
 protected lemma imply₂ : M ⊧ (φ ➝ ψ ➝ χ) ➝ (φ ➝ ψ) ➝ φ ➝ χ := by
   intro x y _ hpqr z Ryz hpq w Rzw hp;
-  have Ryw : y ≺ w := by trans z <;> assumption;
-  have Rww : w ≺ w := by simp;
+  have Ryw : y ≺ w := Frame.rel_trans' Ryz Rzw;
+  have Rww : w ≺ w := Frame.rel_refl';
   exact hpqr Ryw hp Rww (hpq Rzw hp);
 
 protected lemma mdp (hpq : M ⊧ φ ➝ ψ) (hp : M ⊧ φ) : M ⊧ ψ := by
   intro w;
-  exact hpq w Frame.rel_refl $ hp w;
-
-protected lemma bot : ¬M ⊧ ⊥ := by simp [ValidOnModel, Satisfies];
-
-instance : Semantics.Bot (Kripke.Model) := ⟨λ _ => ValidOnModel.bot⟩
+  exact hpq w Frame.rel_refl' $ hp w;
 
 protected lemma efq : M ⊧ Axioms.EFQ φ := by simp [ValidOnModel, Satisfies];
 
-protected lemma neg_equiv : M ⊧ Axioms.NegEquiv φ := by
-  simp_all [ValidOnModel, Axioms.NegEquiv];
-  intro w;
-  constructor;
-  . intro x _ h y rxy hyp; exact h rxy hyp;
-  . intro x _ h y rxy; exact h rxy;
-
 protected lemma lem : Symmetric M.Rel → M ⊧ Axioms.LEM φ := by
-  simp_all [ValidOnModel, Satisfies, Symmetric];
-  contrapose; push_neg;
-  rintro ⟨x, nhxp, ⟨y, Rxy, hyp⟩⟩;
+  unfold Symmetric Axioms.LEM;
+  contrapose;
+  push_neg;
+  intro h;
+  obtain ⟨x, ⟨hnxφ, ⟨y, Rxy, hyφ⟩⟩⟩ := by simpa [Satisfies] using exists_world_of_not h;
   use x, y;
   constructor;
-  . exact Rxy;
+  . assumption;
   . by_contra Ryx;
-    have := formula_hereditary Ryx hyp;
+    have : x ⊧ φ := formula_hereditary Ryx hyφ;
     contradiction;
 
 protected lemma dum : Connected M.Rel → M ⊧ Axioms.Dummett φ ψ := by
-  simp [ValidOnModel, Satisfies, Connected];
-  contrapose; push_neg;
-  rintro ⟨x, ⟨y, Rxy, hyp, nhyq⟩, ⟨z, Ryz, hzq, nhyp⟩⟩;
+  unfold Connected Axioms.Dummett;
+  contrapose;
+  push_neg;
+  intro h;
+  obtain ⟨x, ⟨y, Rxy, hyφ, nhyψ⟩, ⟨z, Ryz, hzψ, nhyφ⟩⟩ := by
+    simpa [Satisfies] using exists_world_of_not h;
   use x, y, z;
-  refine ⟨Rxy, Ryz, ?_, ?_⟩;
+  refine ⟨⟨Rxy, Ryz⟩, ?_, ?_⟩;
   . by_contra Ryz;
-    have := formula_hereditary Ryz hyp;
+    have : z ⊧ φ := formula_hereditary Ryz hyφ;
     contradiction;
   . by_contra Rzy;
-    have := formula_hereditary Rzy hzq;
+    have : y ⊧ ψ := formula_hereditary Rzy hzψ;
     contradiction;
 
 protected lemma wlem : Confluent M.Rel → M ⊧ Axioms.WeakLEM φ := by
-  simp [ValidOnModel, Satisfies, Confluent];
-  contrapose; push_neg;
-  rintro ⟨x, ⟨y, Rxy, hyp⟩, ⟨z, Rxz, hz⟩⟩;
+  unfold Confluent Axioms.WeakLEM;
+  contrapose;
+  push_neg;
+  intro h;
+  obtain ⟨x, ⟨y, Rxy, hyφ⟩, ⟨z, Rxz, hz⟩⟩ := by
+    simpa [Satisfies] using exists_world_of_not h;
   use x, y, z;
-  refine ⟨Rxy, Rxz, ?_⟩;
-  rintro w Ryw;
-  by_contra Rzw;
-  have := formula_hereditary Ryw hyp;
-  have := hz w Rzw;
-  contradiction;
+  refine ⟨⟨Rxy, Rxz⟩, ?_⟩;
+  . rintro w Ryw;
+    by_contra Rzw;
+    have : w ⊧ φ := formula_hereditary Ryw hyφ;
+    have : ¬w ⊧ φ := hz w Rzw;
+    contradiction;
 
 end ValidOnModel
 
 
-def ValidOnFrame (F : Frame) (φ : Formula ℕ) := ∀ {V}, (⟨F, V⟩ : Kripke.Model) ⊧ φ
+def ValidOnFrame (F : Frame) (φ : Formula ℕ) := ∀ V, (⟨F, V⟩ : Kripke.Model) ⊧ φ
 
 
 namespace ValidOnFrame
@@ -251,39 +281,7 @@ variable {F : Frame} {φ ψ χ : Formula ℕ}
 
 @[simp] protected lemma models_iff : F ⊧ φ ↔ ValidOnFrame F φ := iff_of_eq rfl
 
-protected lemma verum : F ⊧ ⊤ := ValidOnModel.verum
-
-protected lemma andElim₁ : F ⊧ φ ⋏ ψ ➝ φ := ValidOnModel.andElim₁
-
-protected lemma andElim₂ : F ⊧ φ ⋏ ψ ➝ ψ := ValidOnModel.andElim₂
-
-protected lemma andInst₃ : F ⊧ φ ➝ ψ ➝ φ ⋏ ψ := ValidOnModel.andInst₃
-
-protected lemma orInst₁ : F ⊧ φ ➝ φ ⋎ ψ := ValidOnModel.orInst₁
-
-protected lemma orInst₂ : F ⊧ ψ ➝ φ ⋎ ψ := ValidOnModel.orInst₂
-
-protected lemma orElim : F ⊧ (φ ➝ χ) ➝ (ψ ➝ χ) ➝ (φ ⋎ ψ ➝ χ) := ValidOnModel.orElim
-
-protected lemma imply₁ : F ⊧ φ ➝ ψ ➝ φ := ValidOnModel.imply₁
-
-protected lemma imply₂ : F ⊧ (φ ➝ ψ ➝ χ) ➝ (φ ➝ ψ) ➝ φ ➝ χ := ValidOnModel.imply₂
-
-protected lemma mdp (hpq : F ⊧ φ ➝ ψ) (hp : F ⊧ φ) : F ⊧ ψ := ValidOnModel.mdp hpq hp
-
-protected lemma efq : F ⊧ Axioms.EFQ φ := ValidOnModel.efq
-
-protected lemma neg_equiv : F ⊧ Axioms.NegEquiv φ := ValidOnModel.neg_equiv
-
-protected lemma lem (F_symm : Symmetric F.Rel) : F ⊧ Axioms.LEM φ := ValidOnModel.lem F_symm
-
-protected lemma dum (F_conn : Connected F.Rel) : F ⊧ Axioms.Dummett φ ψ := ValidOnModel.dum F_conn
-
-protected lemma wlem (F_conf : Confluent F.Rel) : F ⊧ Axioms.WeakLEM φ := ValidOnModel.wlem F_conf
-
-protected lemma top : F ⊧ ⊤ := by
-  simp [ValidOnFrame.models_iff, ValidOnFrame];
-  tauto;
+protected lemma top : F ⊧ ⊤ := by tauto;
 instance : Semantics.Top (Frame) := ⟨λ _ => ValidOnFrame.top⟩
 
 protected lemma bot : ¬F ⊧ ⊥ := by
@@ -291,6 +289,62 @@ protected lemma bot : ¬F ⊧ ⊥ := by
   use ⟨(λ _ _ => True), by tauto⟩;
 instance : Semantics.Bot (Frame) := ⟨λ _ => ValidOnFrame.bot⟩
 
+
+lemma iff_not_exists_valuation : (¬F ⊧ φ) ↔ (∃ V : Kripke.Valuation F, ¬(⟨F, V⟩ : Kripke.Model) ⊧ φ) := by
+  simp [ValidOnFrame];
+
+alias ⟨exists_valuation_of_not, not_of_exists_valuation⟩ := iff_not_exists_valuation
+
+
+lemma iff_not_exists_valuation_world : (¬F ⊧ φ) ↔ (∃ V : Kripke.Valuation F, ∃ x : (⟨F, V⟩ : Kripke.Model).World, ¬Satisfies _ x φ) := by
+  simp [ValidOnFrame, Satisfies, ValidOnModel, Semantics.Realize];
+
+alias ⟨exists_valuation_world_of_not, not_of_exists_valuation_world⟩ := iff_not_exists_valuation_world
+
+
+lemma iff_not_exists_model_world :  (¬F ⊧ φ) ↔ (∃ M : Kripke.Model, ∃ x : M.World, M.toFrame = F ∧ ¬(x ⊧ φ)) := by
+  constructor;
+  . intro h;
+    obtain ⟨V, x, h⟩ := iff_not_exists_valuation_world.mp h;
+    use ⟨F, V⟩, x;
+    tauto;
+  . rintro ⟨M, x, rfl, h⟩;
+    exact iff_not_exists_valuation_world.mpr ⟨M.Val, x, h⟩;
+
+alias ⟨exists_model_world_of_not, not_of_exists_model_world⟩ := iff_not_exists_model_world
+
+
+protected lemma subst (h : F ⊧ φ) : F ⊧ φ⟦s⟧ := by
+  by_contra hC;
+  obtain ⟨V, ⟨x, hx⟩⟩ := exists_valuation_world_of_not hC;
+  apply Satisfies.iff_subst_self s |>.not.mpr hx;
+  apply h;
+
+protected lemma andElim₁ : F ⊧ φ ⋏ ψ ➝ φ := fun _ => ValidOnModel.andElim₁
+
+protected lemma andElim₂ : F ⊧ φ ⋏ ψ ➝ ψ := fun _ => ValidOnModel.andElim₂
+
+protected lemma andInst₃ : F ⊧ φ ➝ ψ ➝ φ ⋏ ψ := fun _ => ValidOnModel.andInst₃
+
+protected lemma orInst₁ : F ⊧ φ ➝ φ ⋎ ψ := fun _ => ValidOnModel.orInst₁
+
+protected lemma orInst₂ : F ⊧ ψ ➝ φ ⋎ ψ := fun _ => ValidOnModel.orInst₂
+
+protected lemma orElim : F ⊧ (φ ➝ χ) ➝ (ψ ➝ χ) ➝ (φ ⋎ ψ ➝ χ) := fun _ => ValidOnModel.orElim
+
+protected lemma imply₁ : F ⊧ φ ➝ ψ ➝ φ := fun _ => ValidOnModel.imply₁
+
+protected lemma imply₂ : F ⊧ (φ ➝ ψ ➝ χ) ➝ (φ ➝ ψ) ➝ φ ➝ χ := fun _ => ValidOnModel.imply₂
+
+protected lemma mdp (hpq : F ⊧ φ ➝ ψ) (hp : F ⊧ φ) : F ⊧ ψ := fun V x => ValidOnModel.mdp (hpq V) (hp V) x
+
+protected lemma efq : F ⊧ Axioms.EFQ φ := fun _ => ValidOnModel.efq
+
+protected lemma lem (F_symm : Symmetric F.Rel) : F ⊧ Axioms.LEM φ := fun _ => ValidOnModel.lem F_symm
+
+protected lemma dum (F_conn : Connected F.Rel) : F ⊧ Axioms.Dummett φ ψ := fun _ => ValidOnModel.dum F_conn
+
+protected lemma wlem (F_conf : Confluent F.Rel) : F ⊧ Axioms.WeakLEM φ := fun _ => ValidOnModel.wlem F_conf
 
 end ValidOnFrame
 
@@ -309,16 +363,116 @@ protected lemma bot (h_nonempty : C.Nonempty) : ¬C ⊧ ⊥ := by
   simp [ValidOnFrameClass.models_iff, ValidOnFrameClass];
   exact h_nonempty;
 
+lemma iff_not_exists_frame {C : Kripke.FrameClass} : (¬C ⊧ φ) ↔ (∃ F ∈ C, ¬F ⊧ φ) := by
+  apply not_iff_not.mp;
+  push_neg;
+  tauto;
+
+alias ⟨exists_frame_of_not, not_of_exists_frame⟩ := iff_not_exists_frame
+
+lemma iff_not_exists_model {C : Kripke.FrameClass} : (¬C ⊧ φ) ↔ (∃ M : Kripke.Model, M.toFrame ∈ C ∧ ¬M ⊧ φ) := by
+  apply not_iff_not.mp;
+  push_neg;
+  tauto;
+
+alias ⟨exists_model_of_not, not_of_exists_model⟩ := iff_not_exists_model
+
+
+lemma iff_not_exists_model_world {C : Kripke.FrameClass} : (¬C ⊧ φ) ↔ (∃ M : Kripke.Model, ∃ x : M.World, M.toFrame ∈ C ∧ ¬(x ⊧ φ)) := by
+  apply not_iff_not.mp;
+  push_neg;
+  tauto;
+
+alias ⟨exists_model_world_of_not, not_of_exists_model_world⟩ := iff_not_exists_model_world
+
 end ValidOnFrameClass
 
 end Formula.Kripke
 
+
+
 namespace Kripke
 
-/--
-  A set of formula that valid on frame `F`.
--/
-def Frame.theorems (F : Kripke.Frame) : Set (Formula ℕ) := { φ | F ⊧ φ }
+namespace FrameClass
+
+variable {C : FrameClass} {φ ψ χ : Formula ℕ}
+
+class DefinedBy (C : Kripke.FrameClass) (Γ : Set (Formula ℕ)) where
+  defines : ∀ F, F ∈ C ↔ (∀ φ ∈ Γ, F ⊧ φ)
+
+class FiniteDefinedBy (C Γ) extends FrameClass.DefinedBy C Γ where
+  finite : Set.Finite Γ
+
+abbrev DefinedByFormula (C : Kripke.FrameClass) (φ : Formula ℕ) := FrameClass.DefinedBy C {φ}
+
+lemma definedByFormula_of_iff_mem_validate (h : ∀ F, F ∈ C ↔ F ⊧ φ) : DefinedByFormula C φ := by
+  constructor;
+  simpa;
+
+instance definedBy_inter
+  (C₁ Γ₁) [h₁ : DefinedBy C₁ Γ₁]
+  (C₂ Γ₂) [h₂ : DefinedBy C₂ Γ₂]
+  : DefinedBy (C₁ ∩ C₂) (Γ₁ ∪ Γ₂) := ⟨by
+  rintro F;
+  constructor
+  . rintro ⟨hF₁, hF₂⟩;
+    rintro φ (hφ₁ | hφ₂);
+    . exact h₁.defines F |>.mp hF₁ _ hφ₁;
+    . exact h₂.defines F |>.mp hF₂ _ hφ₂;
+  . intro h;
+    constructor;
+    . apply h₁.defines F |>.mpr;
+      intro φ hφ;
+      apply h;
+      left;
+      assumption;
+    . apply h₂.defines F |>.mpr;
+      intro φ hφ;
+      apply h;
+      right;
+      assumption;
+⟩
+
+instance definedByFormula_inter
+  (C₁ φ₁) [DefinedByFormula C₁ φ₁]
+  (C₂ φ₂) [DefinedByFormula C₂ φ₂]
+  : DefinedBy (C₁ ∩ C₂) {φ₁, φ₂} := definedBy_inter C₁ {φ₁} C₂ {φ₂}
+
+
+class IsNonempty (C : Kripke.FrameClass) : Prop where
+  nonempty : Nonempty C
+
+end FrameClass
+
+
+abbrev AllFrameClass : FrameClass := Set.univ
+
+instance AllFrameClass.DefinedBy : AllFrameClass.DefinedByFormula (Axioms.EFQ (.atom 0)) :=
+  FrameClass.definedByFormula_of_iff_mem_validate $ by
+    simp only [Set.mem_univ, true_iff];
+    intro F;
+    exact Formula.Kripke.ValidOnFrame.efq;
+
+instance AllFrameClass.IsNonempty : AllFrameClass.IsNonempty := by
+  use pointFrame;
+  trivial;
+
+
+namespace FrameClass
+
+variable {C : Kripke.FrameClass} {Γ : Set (Formula ℕ)}
+
+instance definedBy_with_axiomEFQ (defines : C.DefinedBy Γ) : DefinedBy C (insert (Axioms.EFQ (.atom 0)) Γ) := by
+  convert definedBy_inter AllFrameClass {Axioms.EFQ (.atom 0)} C Γ
+  tauto_set;
+
+end FrameClass
+
+end Kripke
+
+
+/-
+namespace Kripke
 
 def FrameClass.DefinedBy (C : FrameClass) (T : Set (Formula ℕ)) : Prop := ∀ F, F ∈ C ↔ F ⊧* T
 
@@ -517,5 +671,6 @@ instance : (Hilbert.Cl ℕ).Consistent := Kripke.consistent (C := EuclideanFrame
 end Cl
 
 end Hilbert
+-/
 
 end LO.IntProp
