Foundation/IntProp/Kripke/Completeness.lean
@@ -1,13 +1,11 @@
 import Foundation.IntProp.Kripke.Basic
-import Foundation.IntProp.Hilbert.ConsistentTableau
-
-set_option autoImplicit false
-universe u
+import Foundation.IntProp.ConsistentTableau
 
 namespace LO.IntProp
 
-variable {H : Hilbert ℕ}
-variable {t t₁ t₂ : SCT H} {φ ψ : Formula ℕ}
+variable {S} [System (Formula ℕ) S]
+variable {𝓢 : S} [System.Consistent 𝓢] [System.Intuitionistic 𝓢]
+variable {t t₁ t₂ : SaturatedConsistentTableau 𝓢} {φ ψ : Formula ℕ}
 
 open System System.FiniteContext
 open Formula (atom)
@@ -15,187 +13,65 @@ open Formula.Kripke (Satisfies ValidOnModel)
 open Kripke
 open SaturatedConsistentTableau
 
-namespace Hilbert
-
 namespace Kripke
 
-def canonicalFrameOf (H : Hilbert ℕ) [H.Consistent] [H.IncludeEFQ] : Kripke.Frame where
-  World := SCT H
-  Rel t₁ t₂ := t₁.tableau.1 ⊆ t₂.tableau.1
-  rel_po := {
-    refl := by tauto_set;
-    trans := by tauto_set;
-    antisymm := fun x y Sxy Syx => equality_of₁ $ by tauto_set;
-  }
+def canonicalFrame (𝓢 : S) [System.Consistent 𝓢] [System.Intuitionistic 𝓢] : Kripke.Frame where
+  World := SaturatedConsistentTableau 𝓢
+  Rel t₁ t₂ := t₁.1.1 ⊆ t₂.1.1
+  rel_refl := by tauto_set
+  rel_trans := by tauto_set
+    -- antisymm := fun x y Sxy Syx => equality_of₁ $ by tauto_set;
 
 namespace canonicalFrame
 
-variable {H : Hilbert ℕ} [H.IncludeEFQ] [H.Consistent]
-
-open Classical in
-lemma is_confluent [HasAxiomWeakLEM H] : Confluent (Kripke.canonicalFrameOf H) := by
-  simp [Confluent, Kripke.canonicalFrameOf];
-  intro x y z Rxy Rxz;
-  suffices Tableau.Consistent H (y.tableau.1 ∪ z.tableau.1, ∅) by
-    obtain ⟨w, hw⟩ := lindenbaum (H := H) this;
-    use w;
-    simp_all;
-
-  intro Γ Δ;
-  intro hΓ hΔ h;
-  simp_all;
-  have := List.eq_nil_iff_forall_not_mem.mpr hΔ; subst this; simp at h; clear hΔ;
-
-  have hΓy : ¬(∀ w, w ∈ Γ → w ∈ y.tableau.1) := by
-    by_contra hC;
-    have := by simpa using y.consistent (Γ := Γ) (Δ := []) hC (by simp);
-    contradiction;
-  push_neg at hΓy;
-
-  have hΓz : ¬(∀ w, w ∈ Γ → w ∈ z.tableau.1) := by
-    by_contra hC;
-    have := by simpa using z.consistent (Γ := Γ) (Δ := []) hC (by simp);
-    contradiction;
-  push_neg at hΓz;
-
-  let Θy := Γ.filter (λ φ => φ ∈ y.tableau.1 ∧ φ ∉ x.tableau.1);
-  let Θz := Γ.filter (λ φ => φ ∈ z.tableau.1 ∧ φ ∉ x.tableau.1);
-  let Θx := Γ.filter (λ φ => (φ ∈ y.tableau.1 ∧ φ ∈ x.tableau.1) ∨ (φ ∈ z.tableau.1 ∧ φ ∈ x.tableau.1));
-
-  suffices ∼⋀Θy ∈ x.tableau.1 by
-    have : ∼⋀Θy ∈ y.tableau.1 := Rxy this;
-    have : ⋀Θy ∈ y.tableau.1 := iff_mem₁_conj.mpr $ by
-      intro φ hp;
-      have := by simpa using List.of_mem_filter hp;
-      exact this.1;
-    have : H ⊬ ⋀Θy ⋏ ∼⋀Θy ➝ ⊥ := y.consistent (Γ := [⋀Θy, ∼⋀Θy]) (Δ := []) (by simp; constructor <;> assumption) (by simp);
-    have : H ⊢! ⋀Θy ⋏ ∼⋀Θy ➝ ⊥ := intro_bot_of_and!;
-    contradiction;
-
-  have : H ⊢! (⋀Θx ⋏ (⋀Θy ⋏ ⋀Θz)) ➝ ⊥ := imp_trans''! (by
-    -- TODO: need more refactor
-    have d₁ : H ⊢! ⋀Θx ⋏ ⋀(Θy ++ Θz) ➝ ⋀(Θx ++ (Θy ++ Θz)) := and₂'! $ iff_concat_conj!;
-    have d₂ : H ⊢! ⋀Θy ⋏ ⋀Θz ➝ ⋀(Θy ++ Θz) := and₂'! $ iff_concat_conj!;
-    have d₃ : H ⊢! ⋀Θx ⋏ ⋀Θy ⋏ ⋀Θz ➝ ⋀(Θx ++ (Θy ++ Θz)) := imp_trans''! (by
-      apply deduct'!;
-      have : [⋀Θx ⋏ ⋀Θy ⋏ ⋀Θz] ⊢[H]! ⋀Θx ⋏ ⋀Θy ⋏ ⋀Θz := FiniteContext.by_axm!;
-      apply and₃'!;
-      . exact and₁'! this;
-      . exact (FiniteContext.of'! d₂) ⨀ (and₂'! this);
-    ) d₁;
-    exact imp_trans''! d₃ $ conjconj_subset! $ by
-      intro φ hp; simp;
-      apply or_iff_not_imp_left.mpr;
-      intro nmem_Θx;
-      have := (not_imp_not.mpr $ List.mem_filter_of_mem hp) nmem_Θx; simp at this;
-      have ⟨hy₁, hz₁⟩ := this;
-      rcases hΓ _ hp with (hy | hz);
-      . left;
-        apply List.mem_filter_of_mem hp;
-        simp;
-        constructor;
-        . assumption;
-        . exact hy₁ hy;
-      . right;
-        apply List.mem_filter_of_mem hp;
-        simp;
-        constructor;
-        . assumption;
-        . exact hz₁ hz;
-  ) h;
-  have : H ⊢! ⋀Θx ➝ ⋀Θy ➝ ∼⋀Θz := and_imply_iff_imply_imply'!.mp $
-    (imp_trans''! (and_imply_iff_imply_imply'!.mp $ imp_trans''! (and₁'! and_assoc!) this) (and₂'! $ neg_equiv!));
-  have d : H ⊢! ⋀Θx ➝ ∼∼⋀Θz ➝ ∼⋀Θy := imp_trans''! this contra₀!;
-
-  have mem_Θx_x : ⋀Θx ∈ x.tableau.1 := iff_mem₁_conj.mpr $ by
-    intro φ hp;
-    have := by simpa using List.of_mem_filter hp;
-    rcases this with ⟨_, _⟩ | ⟨_, _⟩ <;> assumption;
-  have mem_Θz_z : ⋀Θz ∈ z.tableau.1 := iff_mem₁_conj.mpr $ by
-    intro φ hp;
-    have := by simpa using List.of_mem_filter hp;
-    exact this.1;
-
-  have nmem_nΘz_z : ∼⋀Θz ∉ z.tableau.1 := not_mem₁_neg_of_mem₁ mem_Θz_z;
-  have nmem_nΘz_x : ∼⋀Θz ∉ x.tableau.1 := Set.not_mem_subset Rxz nmem_nΘz_z;
-  have mem_nnΘz_x : ∼∼⋀Θz ∈ x.tableau.1 := or_iff_not_imp_left.mp (iff_mem₁_or.mp $ mem₁_of_provable $ wlem!) nmem_nΘz_x;
-
-  exact mdp₁_mem mem_nnΘz_x $ mdp₁ mem_Θx_x d;
-
-lemma is_connected [HasAxiomDummett H] : Connected (Kripke.canonicalFrameOf H) := by
-  simp [Connected, Kripke.canonicalFrameOf];
-  intro x y z Rxy Ryz;
-  apply or_iff_not_imp_left.mpr;
-  intro nRyz;
-  obtain ⟨φ, hyp, nhzp⟩ := Set.not_subset.mp nRyz;
-  intro ψ hqz;
-  have : ψ ➝ φ ∉ x.tableau.1 := by
-    by_contra hqpx;
-    have hqpz : ψ ➝ φ ∈ z.tableau.1 := by aesop;
-    have : φ ∈ z.tableau.1 := mdp₁_mem hqz hqpz;
-    contradiction;
-  have := iff_mem₁_or.mp $ mem₁_of_provable (t := x) (φ := (φ ➝ ψ) ⋎ (ψ ➝ φ)) dummett!;
-  have hpqx : φ ➝ ψ ∈ x.tableau.1 := by aesop;
-  have hpqy : φ ➝ ψ ∈ y.tableau.1 := Rxy hpqx;
-  have : ψ ∈ y.tableau.1 := mdp₁_mem hyp hpqy;
-  exact this;
+variable [System.Consistent 𝓢] [System.Intuitionistic 𝓢]
 
 end canonicalFrame
 
 
-def canonicalModelOf (H : Hilbert ℕ) [H.Consistent] [H.IncludeEFQ] : Kripke.Model where
-  toFrame := Kripke.canonicalFrameOf H
-  Val := ⟨λ t a => (atom a) ∈ t.tableau.1, by aesop⟩
+def canonicalModel (𝓢 : S) [System.Consistent 𝓢] [System.Intuitionistic 𝓢] : Kripke.Model where
+  toFrame := Kripke.canonicalFrame 𝓢
+  Val := ⟨λ t a => (atom a) ∈ t.1.1, by aesop⟩
 
-/-
-namespace canonicalModelOf
+namespace canonicalModel
 
-variable [Nonempty (SCT H)]
+variable [System.Consistent 𝓢] [System.Intuitionistic 𝓢]
 
-@[reducible]
-instance : Semantics (Formula α) (Kripke.canonicalFrameOf H).World := Formula.Kripke.Satisfies.semantics $ Kripke.canonicalModelOf H
+end canonicalModel
 
-@[simp] lemma frame_def : (Kripke.canonicalModelOf H).toFrame t₁ t₂ ↔ t₁.tableau.1 ⊆ t₂.tableau.1 := by rfl
-@[simp] lemma valuation_def {a : α} : (Kripke.canonicalModelOf H).Valuation t a ↔ (atom a) ∈ t.tableau.1 := by rfl
 
-end canonicalModelOf
--/
-
-section lemmata
-
-variable [H.IncludeEFQ] [H.Consistent]
 variable {C : Kripke.FrameClass}
 
 section truthlemma
 
-variable {t : (Kripke.canonicalModelOf H).World}
+variable {t : (Kripke.canonicalModel 𝓢).World}
 
 private lemma truthlemma.himp
-  (ihp : ∀ {t : (Kripke.canonicalModelOf H).World}, t ⊧ φ ↔ φ ∈ t.tableau.1)
-  (ihq : ∀ {t : (Kripke.canonicalModelOf H).World}, t ⊧ ψ ↔ ψ ∈ t.tableau.1)
-  : t ⊧ φ ➝ ψ ↔ φ ➝ ψ ∈ t.tableau.1 := by
+  (ihp : ∀ {t : (Kripke.canonicalModel 𝓢).World}, t ⊧ φ ↔ φ ∈ t.1.1)
+  (ihq : ∀ {t : (Kripke.canonicalModel 𝓢).World}, t ⊧ ψ ↔ ψ ∈ t.1.1)
+  : t ⊧ φ ➝ ψ ↔ φ ➝ ψ ∈ t.1.1 := by
   constructor;
   . contrapose;
     simp_all [Satisfies];
     intro h;
     replace h := not_mem₁_iff_mem₂.mp h;
-    obtain ⟨t', ⟨h, _⟩⟩ := lindenbaum (H := H) (t₀ := (insert φ t.tableau.1, {ψ})) $ by
+    obtain ⟨t', ⟨h, _⟩⟩ := lindenbaum (𝓢 := 𝓢) (t₀ := (insert φ t.1.1, {ψ})) $ by
       simp only [Tableau.Consistent];
       intro Γ Δ hΓ hΔ;
-      replace hΓ : ∀ χ, χ ∈ Γ.remove φ → χ ∈ t.tableau.1 := by
+      replace hΓ : ∀ χ, χ ∈ Γ.remove φ → χ ∈ t.1.1 := by
         intro χ hr;
         have ⟨hr₁, hr₂⟩ := List.mem_remove_iff.mp hr;
         have := by simpa using hΓ χ hr₁;
         simp_all;
       by_contra hC;
-      have : H ⊢! ⋀(Γ.remove φ) ➝ (φ ➝ ψ) := imp_trans''! (and_imply_iff_imply_imply'!.mp $ imply_left_remove_conj! hC) (by
+      have : 𝓢 ⊢! ⋀(Γ.remove φ) ➝ (φ ➝ ψ) := imp_trans''! (and_imply_iff_imply_imply'!.mp $ imply_left_remove_conj! hC) (by
         apply deduct'!;
         apply deduct!;
-        have : [φ, φ ➝ ⋁Δ] ⊢[H]! φ := by_axm!;
-        have : [φ, φ ➝ ⋁Δ] ⊢[H]! ⋁Δ := by_axm! ⨀ this;
+        have : [φ, φ ➝ ⋁Δ] ⊢[𝓢]! φ := by_axm!;
+        have : [φ, φ ➝ ⋁Δ] ⊢[𝓢]! ⋁Δ := by_axm! ⨀ this;
         exact disj_allsame'! (by simpa using hΔ) this;
       )
-      have : H ⊬ ⋀(Γ.remove φ) ➝ (φ ➝ ψ) := by simpa using (t.consistent hΓ (show ∀ χ ∈ [φ ➝ ψ], χ ∈ t.tableau.2 by simp_all));
+      have : 𝓢 ⊬ ⋀(Γ.remove φ) ➝ (φ ➝ ψ) := by simpa using (t.consistent hΓ (show ∀ χ ∈ [φ ➝ ψ], χ ∈ t.1.2 by simp_all));
       contradiction;
     have ⟨_, _⟩ := Set.insert_subset_iff.mp h;
     use t';
@@ -213,7 +89,7 @@ private lemma truthlemma.himp
     apply not_mem₂_iff_mem₁.mp;
     exact not_mem₂
       (by simp_all)
-      (show H ⊢! ⋀[φ, φ ➝ ψ] ➝ ψ by
+      (show 𝓢 ⊢! ⋀[φ, φ ➝ ψ] ➝ ψ by
         simp;
         apply and_imply_iff_imply_imply'!.mpr;
         apply deduct'!;
@@ -221,57 +97,23 @@ private lemma truthlemma.himp
         exact by_axm! ⨀ (by_axm! (φ := φ));
       );
 
-private lemma truthlemma.hneg
-  (ihp : ∀ {t : (Kripke.canonicalModelOf H).World}, t ⊧ φ ↔ φ ∈ t.tableau.1)
-  : t ⊧ ∼φ ↔ ∼φ ∈ t.tableau.1 := by
-  constructor;
-  . contrapose;
-    simp_all [Satisfies];
-    intro h;
-    replace h := not_mem₁_iff_mem₂.mp h;
-    obtain ⟨t', ⟨h, _⟩⟩ := lindenbaum (H := H) (t₀ := (insert φ t.tableau.1, ∅)) $ by
-      simp only [Tableau.Consistent];
-      intro Γ Δ hΓ hΔ;
-      replace hΓ : ∀ ψ, ψ ∈ Γ.remove φ → ψ ∈ t.tableau.1 := by
-        intro ψ hq;
-        have ⟨hq₁, hq₂⟩ := List.mem_remove_iff.mp hq;
-        have := by simpa using hΓ ψ hq₁;
-        simp_all;
-      replace hΔ : Δ = [] := List.eq_nil_iff_forall_not_mem.mpr hΔ; subst hΔ;
-      by_contra hC; simp at hC;
-      have : H ⊢! ⋀(Γ.remove φ) ➝ ∼φ := imp_trans''! (and_imply_iff_imply_imply'!.mp $ imply_left_remove_conj! hC) (and₂'! neg_equiv!);
-      have : H ⊬ ⋀(Γ.remove φ) ➝ ∼φ := by simpa using t.consistent (Δ := [∼φ]) hΓ (by simpa);
-      contradiction;
-    have ⟨_, _⟩ := Set.insert_subset_iff.mp h;
-    use t';
-    constructor <;> assumption;
-  . simp;
-    intro ht t' htt';
-    apply ihp.not.mpr;
-    by_contra hC;
-    have : H ⊬ φ ⋏ ∼φ ➝ ⊥ := by simpa using t'.consistent (Γ := [φ, ∼φ]) (Δ := []) (by aesop) (by simp);
-    have : H ⊢! φ ⋏ ∼φ ➝ ⊥ := intro_bot_of_and!;
-    contradiction;
-
-lemma truthlemma : t ⊧ φ ↔ φ ∈ t.tableau.1 := by
+lemma truthlemma : t ⊧ φ ↔ φ ∈ t.1.1 := by
   induction φ using Formula.rec' generalizing t with
   | hatom => tauto;
   | himp φ ψ ihp ihq => exact truthlemma.himp ihp ihq;
   | _ => simp [Satisfies.iff_models, Satisfies, *];
 
-end truthlemma
-
-lemma deducible_of_validOnCanonicelModel : (Kripke.canonicalModelOf H) ⊧ φ ↔ H ⊢! φ := by
+lemma iff_valid_on_canonicalModel_deducible : (Kripke.canonicalModel 𝓢) ⊧ φ ↔ 𝓢 ⊢! φ := by
   constructor;
   . contrapose;
     intro h;
-    have : Tableau.Consistent H (∅, {φ}) := by
+    have : Tableau.Consistent 𝓢 (∅, {φ}) := by
       simp only [Tableau.Consistent, Collection.not_mem_empty, imp_false, Set.mem_singleton_iff];
       rintro Γ Δ hΓ hΔ;
       by_contra hC;
       replace hΓ : Γ = [] := List.eq_nil_iff_forall_not_mem.mpr hΓ;
       subst hΓ;
-      have : H ⊢! φ := disj_allsame'! hΔ (hC ⨀ verum!);
+      have : 𝓢 ⊢! φ := disj_allsame'! hΔ (hC ⨀ verum!);
       contradiction;
     obtain ⟨t', ht'⟩ := lindenbaum this;
     simp [ValidOnModel.iff_models, ValidOnModel]
@@ -280,32 +122,23 @@ lemma deducible_of_validOnCanonicelModel : (Kripke.canonicalModelOf H) ⊧ φ �
     apply not_mem₁_iff_mem₂.mpr;
     simp_all;
   . intro h t;
-    suffices φ ∈ t.tableau.1 by exact truthlemma.mpr this;
+    suffices φ ∈ t.1.1 by exact truthlemma.mpr this;
     exact mem₁_of_provable h;
 
-lemma complete_of_canonical (hC : (Kripke.canonicalFrameOf H) ∈ C) : C ⊧ φ → H ⊢! φ := by
-  intro h;
-  apply deducible_of_validOnCanonicelModel.mp;
+end truthlemma
+
+
+class Canonical (𝓢 : S) [System.Consistent 𝓢] [System.Intuitionistic 𝓢] (C : FrameClass) : Prop where
+  canonical : (Kripke.canonicalFrame 𝓢) ∈ C
+
+instance instCompleteOfCanonical [Canonical 𝓢 C] : Complete 𝓢 C := ⟨by
+  intro φ h;
+  apply iff_valid_on_canonicalModel_deducible.mp;
   apply h;
-  exact hC;
+  exact Canonical.canonical;
+⟩
 
-instance instCompleteOfCanonical (hC : (Kripke.canonicalFrameOf H) ∈ C) : Complete H C := ⟨complete_of_canonical hC⟩
-
-end lemmata
 
 end Kripke
-
-
-section completeness
-
-instance Int.Kripke.complete : Complete (Hilbert.Int ℕ) AllFrameClass := Hilbert.Kripke.instCompleteOfCanonical $ by tauto
-
-instance KC.Kripke.complete : Complete (Hilbert.KC ℕ) ConfluentFrameClass := Hilbert.Kripke.instCompleteOfCanonical $ Kripke.canonicalFrame.is_confluent
-
-instance LC.Kripke.complete : Complete (Hilbert.LC ℕ) ConnectedFrameClass := Hilbert.Kripke.instCompleteOfCanonical $ Kripke.canonicalFrame.is_connected
-
-end completeness
-
-end Hilbert
 
 end LO.IntProp
