Foundation/IntProp/Hilbert/Glivenko.lean
@@ -1,5 +1,5 @@
 import Foundation.Logic.HilbertStyle.Supplemental
-import Foundation.IntProp.Hilbert.Basic
+import Foundation.IntProp.Hilbert.WellKnown
 
 namespace LO.IntProp
 
@@ -9,28 +9,31 @@ open System
 
 variable [DecidableEq α]
 
-theorem iff_provable_dn_efq_dne_provable : (Hilbert.Int α) ⊢! ∼∼φ ↔ (Hilbert.Cl α) ⊢! φ := by
+theorem iff_provable_dn_efq_dne_provable : (Hilbert.Int) ⊢! ∼∼φ ↔ (Hilbert.Cl) ⊢! φ := by
   constructor;
-  . intro d; exact dne'! $ Int_weaker_than_Cl d;
+  . intro d; exact dne'! $ Int_weakerThan_Cl d;
   . intro d;
     induction d using Deduction.rec! with
-    | eaxm hp =>
-      rcases hp with (⟨_, rfl⟩ | ⟨ψ, rfl⟩);
-      . apply dni'!; exact efq!;
-      . apply neg_equiv'!.mpr;
+    | maxm hp =>
+      rcases (by simpa using hp) with (⟨_, rfl⟩ | ⟨s, rfl⟩);
+      . apply dni'!;
+        exact efq!;
+      . generalize (s 0) = ψ;
+        apply neg_equiv'!.mpr;
         apply FiniteContext.deduct'!;
-        have : [∼(ψ ⋎ ∼ψ)] ⊢[Hilbert.Int α]! ∼ψ ⋏ ∼∼ψ := demorgan₃'! $ FiniteContext.id!;
-        exact neg_mdp! (and₂'! this) (and₁'! this);
-    | mdp ihφψ ihφ =>
-      exact dn_distribute_imply'! ihφψ ⨀ ihφ;
+        have : [∼(ψ ⋎ (ψ ➝ ⊥))] ⊢[Hilbert.Int]! ∼ψ ⋏ ∼(ψ ➝ ⊥) := demorgan₃'! $ FiniteContext.id!;
+        exact (neg_equiv'!.mp $ and₂'! this) ⨀ (neg_equiv'!.mp $ and₁'! this);
+    | mdp ihφψ ihφ => exact dn_distribute_imply'! ihφψ ⨀ ihφ;
     | _ => apply dni'!; simp;
 
 alias glivenko := iff_provable_dn_efq_dne_provable
 
-theorem iff_provable_neg_efq_provable_neg_efq : (Hilbert.Int α) ⊢! ∼φ ↔ (Hilbert.Cl α) ⊢! ∼φ := by
+theorem iff_provable_neg_efq_provable_neg_efq : (Hilbert.Int) ⊢! ∼φ ↔ (Hilbert.Cl) ⊢! ∼φ := by
   constructor;
-  . intro d; exact glivenko.mp $ dni'! d;
-  . intro d; exact tne'! $ glivenko.mpr d;
+  . intro d;
+    exact glivenko.mp $ dni'! d;
+  . intro d;
+    exact tne'! $ glivenko.mpr d;
 
 end Hilbert
 
