Foundation/IntProp/Kripke/Hilbert/Cl/Basic.lean
@@ -1,5 +1,5 @@
-import Foundation.IntProp.Hilbert2.WellKnown
-import Foundation.IntProp.Kripke2.Hilbert.Soundness
+import Foundation.IntProp.Hilbert.WellKnown
+import Foundation.IntProp.Kripke.Hilbert.Soundness
 
 namespace LO.IntProp
 
