Foundation/Modal/ModalCompanion/Basic.lean
@@ -1,5 +1,5 @@
 import Foundation.Logic.Disjunctive
-import Foundation.IntProp.Hilbert.Basic
+import Foundation.IntProp.Hilbert.WellKnown
 import Foundation.Modal.Hilbert.WellKnown
 
 namespace LO.Modal
@@ -38,11 +38,11 @@ lemma axiomTc_GTranslate! [System.K4 mH] : mH ⊢! φᵍ ➝ □φᵍ := by
 section
 
 private lemma provable_efq_of_provable_S4.case_imply₁ [System.K4 mH] : mH ⊢! (φ ➝ ψ ➝ φ)ᵍ := by
-  simp only [GoedelTranslation];
+  dsimp [GoedelTranslation];
   exact nec! $ imp_trans''! axiomTc_GTranslate! $ axiomK'! $ nec! $ imply₁!;
 
 private lemma provable_efq_of_provable_S4.case_imply₂ [System.S4 mH] : mH ⊢! ((φ ➝ ψ ➝ χ) ➝ (φ ➝ ψ) ➝ φ ➝ χ)ᵍ := by
-  simp only [GoedelTranslation];
+  dsimp [GoedelTranslation];
   apply nec! $ imp_trans''! (imp_trans''! (axiomK'! $ nec! ?b) axiomFour!) $ axiomK'! $ nec! $ imp_trans''! (axiomK'! $ nec! imply₂!) axiomK!;
   apply provable_iff_provable.mpr;
   apply deduct_iff.mpr;
@@ -52,37 +52,30 @@ private lemma provable_efq_of_provable_S4.case_imply₂ [System.S4 mH] : mH ⊢!
   have : [φᵍ, φᵍ ➝ □(ψᵍ ➝ χᵍ)] ⊢[mH]! □(ψᵍ ➝ χᵍ) := (by assumption) ⨀ (by assumption);
   exact axiomT'! this;
 private lemma provable_efq_of_provable_S4.case_and₃ [System.K4 mH] : mH ⊢! (φ ➝ ψ ➝ φ ⋏ ψ)ᵍ := by
-  simp only [GoedelTranslation];
+  dsimp [GoedelTranslation];
   exact nec! $ imp_trans''! axiomTc_GTranslate! $ axiomK'! $ nec! $ and₃!
 
 private lemma provable_efq_of_provable_S4.case_or₃ [System.K4 mH] : mH ⊢! (((φ ➝ χ) ➝ (ψ ➝ χ) ➝ (φ ⋎ ψ ➝ χ)))ᵍ := by
-  simp only [GoedelTranslation];
+  dsimp [GoedelTranslation];
   exact nec! $ imp_trans''! axiomFour! $ axiomK'! $ nec! $ imp_trans''! (axiomK'! $ nec! $ or₃!) axiomK!;
 
-private lemma provable_efq_of_provable_S4.case_neg_equiv [System.K4 mH] : mH ⊢! (Axioms.NegEquiv φ)ᵍ := by
-  simp only [GoedelTranslation];
-  apply and₃'!;
-  . exact nec! $ axiomK'! $ nec! $ and₁'! neg_equiv!;
-  . exact nec! $ axiomK'! $ nec! $ and₂'! neg_equiv!;
-
 open provable_efq_of_provable_S4 in
-lemma provable_efq_of_provable_S4 (h : (Hilbert.Int _) ⊢! φ) : (Hilbert.S4) ⊢! φᵍ := by
-  induction h.some with
-  | eaxm ih =>
-    simp_all only [Set.mem_setOf_eq];
-    obtain ⟨φ, hp⟩ := ih; subst hp;
+lemma provable_efq_of_provable_S4 (h : (IntProp.Hilbert.Int) ⊢! φ) : (Hilbert.S4) ⊢! φᵍ := by
+  induction h using IntProp.Hilbert.Deduction.rec! with
+  | maxm ih =>
+    rcases (by simpa using ih) with ⟨_, rfl⟩;
     exact nec! efq!;
-  | mdp hpq hp ihpq ihp =>
-    exact axiomT'! $ axiomK''! (by simpa using ihpq ⟨hpq⟩) $ nec! $ ihp ⟨hp⟩;
-  | and₁ => exact nec! and₁!;
-  | and₂ => exact nec! and₂!;
-  | or₁ => exact nec! or₁!;
-  | or₂ => exact nec! or₂!;
+  | mdp ihpq ihp =>
+    exact axiomT'! $ axiomK''! (ihpq) $ nec! $ ihp;
   | verum => exact nec! imp_id!;
-  | imply₁ => exact case_imply₁;
-  | imply₂ => exact case_imply₂;
-  | and₃ => exact case_and₃;
-  | or₃ => exact case_or₃;
+  | andElimL => exact nec! and₁!;
+  | andElimR => exact nec! and₂!;
+  | andIntro => exact case_and₃;
+  | orIntroL => exact nec! or₁!;
+  | orIntroR => exact nec! or₂!;
+  | orElim => exact case_or₃;
+  | implyS => exact case_imply₁;
+  | implyK => exact case_imply₂;
 
 end
 
